track sum

rocq-brick-libstdcpp/proof/mutex/demo_cpp_proof.v
@@ -7,21 +7,36 @@ Section with_cpp.
   Context `{Σ : cpp_logic}.
   Context `{MOD : source ⊧ σ}. (* σ is the whole program *)
   Context {has_rmutex : HasOwn mpredI (excl_authR natO)}.
+  Implicit Type (s: Z).
 
-  Definition TT : tele := [tele (_ : Z) (_ : Z)].
-  Definition mk (a b : Z) : TT :=
-    {| tele_arg_head := a; tele_arg_tail := {| tele_arg_head := b; tele_arg_tail := () |} |}.
+  Record R := mk_R {
+    a : Z;
+    b : Z;
+    y : bool;
+  }.
 
-  Definition P (this : ptr) : TT -t> mpred :=
-    fun (a b : Z) =>
-       this ,, _field "C::balance_a" |-> intR 1$m a **
-       this ,, _field "C::balance_b" |-> intR 1$m b.
+  (* maybe simpler if we only have one layer of tele? *)
+  Definition TT : tele := [tele (_ : R)].
 
-  Definition CR (γ : gname) (q : cQp.t) : Rep :=
+  Definition mk (r : R) : TT :=
+    {| tele_arg_head := r; tele_arg_tail := () |}.
+
+  Definition r_of (args:TT) : R :=
+    (tele_arg_head _ args).
+
+  Definition P (this : ptr) (maybe_s:option Z) : TT -t> mpred :=
+    fun (r : R) =>
+       this ,, _field "C::balance_a" |-> intR 1$m r.(a) **
+       this ,, _field "C::balance_b" |-> intR 1$m r.(b) **
+       match maybe_s with 
+       | Some s => if r.(y) then [| (r.(a)+r.(b))%Z = s |] else emp
+       | None => emp end.
+
+  Definition CR (γ : gname) (q : cQp.t) maybe_s : Rep :=
     structR "C" q **
     _field "C::mut" |-> recursive_mutex.R γ q **
     as_Rep (fun this : ptr =>
-      recursive_mutex.inv_rmutex γ (∃ a_b : tele_arg _, tele_app (P this) a_b)).
+      recursive_mutex.inv_rmutex γ (∃ (r : tele_arg _), tele_app (P this maybe_s) r)).
 
   Definition update {TT : tele} (f : TT -t> TT)
     (x : @recursive_mutex.acquire_state TT)
@@ -31,76 +46,163 @@ Section with_cpp.
     | recursive_mutex.Held n xs => recursive_mutex.Held n (tele_app f xs)
     end.
 
-  cpp.spec "C::update_a(int)" with
-    (\this this
-     \arg{x} "x" (Vint x)
-     \prepost{γ q} this |-> CR γ q
-     \pre{args th} recursive_mutex.acquireable γ th args (TT:=TT) (P this)
-     \post recursive_mutex.acquireable γ th (TT:=TT) (update (TT:=TT) (fun (a b : Z) => mk (a+x) b) args) (P this)).
-
-  cpp.spec "C::update_b(int)" with
-    (\this this
-     \arg{x} "x" (Vint x)
-     \prepost{γ q} this |-> CR γ q
-     \pre{args th} recursive_mutex.acquireable γ th args (TT:=TT) (P this)
-     \post recursive_mutex.acquireable γ th (TT:=TT) (update (TT:=TT) (fun (a b : Z) => mk a (b + x)) args) (P this)).
-
   #[global] Instance acquireable_learn γ th TT : LearnEq2 (@recursive_mutex.acquireable _ _ _ γ th TT).
-  Proof. solve_learnable. Qed.
+    Proof. solve_learnable. Qed.
 
-  Lemma update_a_ok : verify[source] "C::update_a(int)".
-  Proof.
-    verify_spec; go.
-    rewrite /CR.
-    iExists _; iExists TT; iExists (P this); iExists q; iExists th.
-    go. ego.
-    destruct args.
-    { simpl in *. destruct H; subst.
-      go.
-      rewrite /P/=. destruct x0 as [?[? []]]; simpl.
-      go.
-      iSplitR. { admit. }
-      go.
-      iExists γ; iExists TT; iExists (P this); iExists q; iExists th; iExists 0; iExists (mk (_ + x) _).
-      go. rewrite /P. go. }
-    {  simpl in *. subst.
-       rewrite /P/=. destruct xs as [a [b []]]; simpl.
-       go.
-       iSplitR. { admit. }
-       go.
-       iExists γ; iExists TT; iExists (P this); iExists q; iExists th; iExists (S n); iExists (mk (_ + x) _).
-       go. rewrite /P. go.
-       rewrite /P. go. }
-  Admitted.
+  Section A_PLUS_B_INV.
 
-  cpp.spec "C::transfer(int)" with
-    (\this this
+    cpp.spec "C::update_a(int)" with
+      (\this this
       \arg{x} "x" (Vint x)
-      \prepost{γ q} this |-> CR γ q
-      \pre{args th} recursive_mutex.acquireable γ th args (TT:=TT) (P this)
-      \post recursive_mutex.acquireable γ th (TT:=TT) (update (TT:=TT) (fun (a b : Z) => mk (a+x) (b-x)) args) (P this)).
+      \prepost{γ q s} this |-> CR γ q (Some s)
+      \pre{st th n args} recursive_mutex.acquireable γ th st (TT:=TT) (P this (Some s)) **
+                         [| st = recursive_mutex.Held n args |] **
+                         (* [| (0 <= a (r_of args) + x)%Z |] ** (* can't transfer beyond balance *) *)
+                         [| valid<"int"> (a (r_of args) + x)%Z |] (* user responsible for overflow *)
+      \post recursive_mutex.acquireable γ th (TT:=TT) (update (TT:=TT) (fun (r : R) => mk $ mk_R (a r + x) (b r) false) st)
+        (P this $ (Some s))).
 
-  Opaque recursive_mutex.acquireable.
-  Lemma transfer_ok : verify[source] "C::transfer(int)".
-  Proof.
-    verify_spec; go.
-    rewrite /CR. go.
-    iExists γ; iExists TT; iExists (P this); iExists q; iExists th; iExists _. go.
-    { ego. }
-    iExists γ; iExists q; iExists _; iExists th; go.
-    { ego. }
-    rewrite /CR.
-    iExists γ; iExists q; iExists _; iExists th; go.
-    iSplitL; [ | admit ].
-    go.
-    destruct args.
-    { destruct H. subst.
-      iExists γ; iExists TT; iExists (P this); iExists q; iExists th; iExists _; iExists _. go. }
-    { red in H; subst.
-      iExists γ; iExists TT; iExists (P this); iExists q; iExists th; iExists _; iExists _. go.
-      destruct xs as [a[b[]]]; simpl.
-      have->: (b + (0 - x) = b - x)%Z by lia.
-      go. }
-  Admitted.
+    cpp.spec "C::update_b(int)" with
+      (\this this
+      \arg{x} "x" (Vint x)
+      \prepost{γ q s} this |-> CR γ q (Some s)
+      \pre{st th n args} recursive_mutex.acquireable γ th st (TT:=TT) (P this (Some s)) **
+                         [| st = recursive_mutex.Held n args |] **
+                         (* [| (0 <= b (r_of args) + x)%Z |] ** (* can't transfer beyond balance *) *)
+                         [| valid<"int"> (b (r_of args) + x)%Z |] (* user responsible for overflow *)
+      \post recursive_mutex.acquireable γ th (TT:=TT) (update (TT:=TT) (fun (r : R) => mk $ mk_R (a r) (b r + x) false) st)
+        (P this $ (Some s))).
+
+
+    Lemma update_a_ok : verify[source] "C::update_a(int)".
+    Proof using MOD _Σ has_rmutex thread_info Σ σ.
+      verify_spec; go.
+      rewrite /CR.
+      iExists _; iExists TT; iExists (P this (Some s)); iExists q; iExists th; iExists (recursive_mutex.Held n args).
+      go. ego.
+      rewrite /P/=. destruct args as [r[]]; simpl.
+      go.
+      iExists _; iExists TT. iExists (P this $ Some s)%Z; iExists q; iExists th. iExists (S n); iExists (mk $ mk_R (_ + x) _ false).
+      go.
+      rewrite /P/=. go.
+      rewrite /P/=. go.
+    Qed.
+
+    cpp.spec "C::transfer(int)" with
+      (\this this
+        \arg{x} "x" (Vint x)
+        \prepost{γ q s} this |-> CR γ q (Some s)
+        \pre{st th} recursive_mutex.acquireable γ th st (TT:=TT) (P this $ Some s)
+        \post recursive_mutex.acquireable γ th (TT:=TT) (update (TT:=TT) (fun (r : R) => mk $ mk_R (r.(a)+x) (r.(b)-x) true) st) (P this $ Some s)).
+
+    Lemma transfer_ok : verify[source] "C::transfer(int)".
+    Proof.
+      verify_spec; go.
+      rewrite /CR. go.
+      iExists γ; iExists TT; iExists (P this $ Some s); iExists q; iExists th; iExists _. go.
+      { ego. }
+      assert (∃ n args, t = recursive_mutex.Held n args) as [n [args Ht]].
+      {  rewrite /recursive_mutex.acquire in H. destruct st; [destruct H as [? ?] | subst]; eexists; eauto. }
+      iExists γ; iExists q; iExists s; iExists n; iExists th; iExists args; go.
+      subst; simpl. go.
+      iSplitR; first admit.
+      go. ego.
+      iExists γ; iExists q; iExists s; iExists n; iExists th; iExists _; go.
+      rewrite /CR/=. go.
+      iSplit; last admit.
+      go. iFrame.
+      go.
+      iSplit; first admit.
+      go.
+      iExists γ; iExists TT; iExists (P this $ Some s); iExists q; iExists th; iExists _; iExists _. go.
+      iFrame. go.
+      rewrite /recursive_mutex.acquire in H.
+      destruct st.
+      { 
+        destruct H. inversion H; subst.
+        simpl. done.
+      }
+      {
+        inversion H; subst.
+        rewrite /P/=. 
+        destruct xs as [args[]].
+        destruct args. simpl.
+        go. iPureIntro. admit.  
+      }
+    Admitted.
+  End A_PLUS_B_INV.
+
+  (* original version, do not enforce a+b to stay the same when lock is not held *)
+  Section A_PLUS_B_NOT_INV.
+    (* FIXME need to give it another name *)
+    cpp.spec "C::update_a(int)" with
+      (\this this
+      \arg{x} "x" (Vint x)
+      \prepost{γ q} this |-> CR γ q None
+      \pre{args th} recursive_mutex.acquireable γ th args (TT:=TT) (P this None)
+      \post recursive_mutex.acquireable γ th (TT:=TT) (update (TT:=TT) (fun (r : R) => mk $ mk_R (r.(a) + x) r.(b)) args) (P this None)).
+
+    cpp.spec "C::update_b(int)" with
+      (\this this
+      \arg{x} "x" (Vint x)
+      \prepost{γ q} this |-> CR γ q None
+      \pre{args th} recursive_mutex.acquireable γ th args (TT:=TT) (P this None)
+      \post recursive_mutex.acquireable γ th (TT:=TT) (update (TT:=TT) (fun (r : R) => mk $ mk_R r.(a) (r.(b) + x)) args) (P this None)).
+
+    Lemma update_a_ok : verify[source] "C::update_a(int)".
+    Proof.
+      verify_spec; go.
+      rewrite /CR.
+      iExists _; iExists TT; iExists (P this None); iExists q; iExists th.
+      go. ego.
+      destruct args.
+      { simpl in *. destruct H; subst.
+        go.
+        rewrite /P/=. destruct x0 as [r[]]; simpl.
+        go.
+        iSplitR. { admit. }
+        go.
+        iExists γ; iExists TT; iExists (P this None); iExists q; iExists th; iExists 0; iExists (mk $ mk_R (_ + x) _).
+        go. rewrite /P. go. }
+      {  simpl in *. subst.
+        rewrite /P/=. destruct xs as [r[]]; simpl.
+        go.
+        iSplitR. { admit. }
+        go.
+        iExists γ; iExists TT; iExists (P this None); iExists q; iExists th; iExists (S n); iExists (mk $ mk_R (_ + x) _).
+        go. rewrite /P. go.
+        rewrite /P. go. }
+    Admitted.
+
+    cpp.spec "C::transfer(int)" with
+      (\this this
+        \arg{x} "x" (Vint x)
+        \prepost{γ q} this |-> CR γ q None
+        \pre{args th} recursive_mutex.acquireable γ th args (TT:=TT) (P this None)
+        \post recursive_mutex.acquireable γ th (TT:=TT) (update (TT:=TT) (fun (r : R) => mk $ mk_R (r.(a)+x) (r.(b)-x)) args) (P this None)).
+
+    Opaque recursive_mutex.acquireable.
+    Lemma transfer_ok : verify[source] "C::transfer(int)".
+    Proof.
+      verify_spec; go.
+      rewrite /CR. go.
+      iExists γ; iExists TT; iExists (P this None); iExists q; iExists th; iExists _. go.
+      { ego. }
+      iExists γ; iExists q; iExists _; iExists th; go.
+      { ego. }
+      rewrite /CR.
+      iExists γ; iExists q; iExists _; iExists th; go.
+      iSplitL; [ | admit ].
+      go.
+      destruct args.
+      { destruct H. subst.
+        iExists γ; iExists TT; iExists (P this None); iExists q; iExists th; iExists _; iExists _. go. }
+      { red in H; subst.
+        iExists γ; iExists TT; iExists (P this None); iExists q; iExists th; iExists _; iExists _. go.
+        destruct xs as [r[]]; simpl.
+        have->: (b r + (0 - x) = b r - x)%Z by lia.
+        go. }
+    Admitted.
+  End A_PLUS_B_NOT_INV.
 
 End with_cpp.
